coq/Parsing.v
@@ -128,18 +128,18 @@ Notation "a '[' b ']'" := (UBinop (UBits2 USel) a b) (in custom koika at level 7
 Notation "a '[' b ':+' c ']'" := (UBinop (UBits2 (UIndexedSlice c)) a b) (in custom koika at level 75, c constr at level 0, format "'[' a [ b ':+' c ] ']'").
 Notation "'`' a '`'" := ( a) (in custom koika at level 99, a constr at level 99).
 
-Notation "'fun' args ':' ret '=>' body" :=
-  {| int_name := "";
+Notation "'fun' nm args ':' ret '=>' body" :=
+  {| int_name := nm%string;
      int_argspec := args;
      int_retSig := ret;
      int_body := body |}
-    (in custom koika at level 99, args custom koika_types, ret constr at level 0, body custom koika at level 99, format "'[v' 'fun'  args  ':'  ret  '=>' '/' body ']'").
-Notation "'fun' '_' ':' ret '=>' body" :=
-  {| int_name := "";
+    (in custom koika at level 99, nm custom koika_var at level 0, args custom koika_types, ret constr at level 0, body custom koika at level 99, format "'[v' 'fun'  nm  args  ':'  ret  '=>' '/' body ']'").
+Notation "'fun' nm '()' ':' ret '=>' body" :=
+  {| int_name := nm%string;
      int_argspec := nil;
      int_retSig := ret;
      int_body := body |}
-    (in custom koika at level 99,  ret constr at level 0, body custom koika at level 99, format "'[v' 'fun'  '_'   ':'  ret  '=>' '/' body ']'").
+    (in custom koika at level 99, nm custom koika_var at level 0, ret constr at level 0, body custom koika at level 99, format "'[v' 'fun'  nm  '()'   ':'  ret  '=>' '/' body ']'").
 
 (* Deprecated *)
 Notation "'call' instance method args" :=
@@ -152,7 +152,7 @@ Notation "'extcall' method '(' arg ')'" :=
   (UExternalCall method arg)
     (in custom koika at level 98, method constr at level 0, arg custom koika).
 Notation "'call0' instance method " :=
-  (UCallModule instance id method nil)
+  (USugar (UCallModule instance id method nil))
     (in custom koika at level 98, instance constr at level 0, method constr).
 Notation "'funcall0' method " :=
   (UInternalCall method nil)
@@ -242,10 +242,10 @@ Module Type Tests.
   (* Notation "'{&' a '&}'" := (a) (a custom koika_types at level 200). *)
   (* Definition test_21 := {& "yoyo" : bits_t 2 &}. *)
   (* Definition test_22 := {& "yoyo" : bits_t 2 , "yoyo" : bits_t 2  &}. *)
-  Definition test_23 : InternalFunction string string (uaction reg_t) := {{ fun (arg1 : (bits_t 3)) (arg2 : bits_t 2) : bits_t 4 => magic }}.
-  Definition test_24 : nat -> InternalFunction string string (uaction reg_t) :=  (fun sz => {{ fun  (arg1 : bits_t sz) (arg1 : bits_t sz) : bits_t sz  => magic}}).
-  Definition test_25 : nat -> InternalFunction string string (uaction reg_t) := (fun sz => {{fun (arg1 : bits_t sz ) : bits_t sz => let oo := magic >> magic in magic}}).
-  Definition test_26 : nat -> InternalFunction string string (uaction reg_t) := (fun sz => {{ fun _ : bits_t sz  => magic }}).
+  Definition test_23 : InternalFunction string string (uaction reg_t) := {{ fun test (arg1 : (bits_t 3)) (arg2 : bits_t 2) : bits_t 4 => magic }}.
+  Definition test_24 : nat -> InternalFunction string string (uaction reg_t) :=  (fun sz => {{ fun test (arg1 : bits_t sz) (arg1 : bits_t sz) : bits_t sz  => magic}}).
+  Definition test_25 : nat -> InternalFunction string string (uaction reg_t) := (fun sz => {{fun test (arg1 : bits_t sz ) : bits_t sz => let oo := magic >> magic in magic}}).
+  Definition test_26 : nat -> InternalFunction string string (uaction reg_t) := (fun sz => {{ fun test () : bits_t sz  => magic }}).
   Definition test_27 : uaction reg_t :=
     {{
         (if (!read0(data0)) then
