coq/Syntax.v
@@ -18,7 +18,7 @@ Section Syntax.
   | UUnop (ufn1: PrimUntyped.ufn1) (arg1: uaction)
   | UBinop (ufn2: PrimUntyped.ufn2) (arg1: uaction) (arg2: uaction)
   | UExternalCall (ufn: ext_fn_t) (arg: uaction)
-  | UInternalCall (ufn: InternalFunction fn_name_t var_t uaction) (args: list uaction)
+  | UInternalCall (ufn: InternalFunction var_t fn_name_t uaction) (args: list uaction)
   | UAPos (p: pos_t) (e: uaction)
   | USugar (s: usugar)
   with usugar {reg_t ext_fn_t} :=
@@ -38,7 +38,7 @@ Section Syntax.
   | UCallModule {module_reg_t module_ext_fn_t: Type}
                 (fR: module_reg_t -> reg_t)
                 (fSigma: module_ext_fn_t -> ext_fn_t)
-                (fn: InternalFunction fn_name_t var_t (@uaction module_reg_t module_ext_fn_t))
+                (fn: InternalFunction var_t fn_name_t (@uaction module_reg_t module_ext_fn_t))
                 (args: list uaction).
 
   Inductive scheduler :=
